Mostly finished DNS packet decoder.

src/BinEncoders/Env/Examples/DnsOpt.v
@@ -39,11 +39,11 @@ Section DnsPacket.
   Variable cacheGetDNPointer : CacheGet cache string pointerT.
   Variable cachePeekDNPointer : CachePeek cache pointerT.
 
-  Variable QType_Ws : t (word 16) 66.
+  Variable QType_Ws : t (word 16) 17.
   Variable QType_Ws_OK : NoDupVector QType_Ws.
   Variable QClass_Ws : t (word 16) 4.
   Variable QClass_Ws_OK : NoDupVector QClass_Ws.
-  Variable RRecordType_Ws : t (word 16) 59.
+  Variable RRecordType_Ws : t (word 16) 10.
   Variable RRecordType_Ws_OK : NoDupVector  RRecordType_Ws.
   Variable RRecordClass_Ws : t (word 16) 3.
   Variable RRecordClass_Ws_OK : NoDupVector  RRecordClass_Ws.
@@ -65,8 +65,14 @@ Section DnsPacket.
   ThenC encode_enum_Spec QClass_Ws q!"qclass"
   DoneC.
 
+  Definition encode_TXT_Spec (s : string) :=
+    encode_unused_word_Spec 16 (* Unusued RDLENGTH Field *)
+  ThenC encode_characterString_Spec s
+  DoneC.
+
   Definition encode_SOA_RDATA_Spec (soa : SOA_RDATA) :=
-       encode_DomainName_Spec soa!"sourcehost"
+    encode_unused_word_Spec 16 (* Unusued RDLENGTH Field *)
+  ThenC encode_DomainName_Spec soa!"sourcehost"
   ThenC encode_DomainName_Spec soa!"contact_email"
   ThenC encode_word_Spec soa!"serial"
   ThenC encode_word_Spec soa!"refresh"
@@ -76,44 +82,68 @@ Section DnsPacket.
   DoneC.
 
   Definition encode_WKS_RDATA_Spec (wks : WKS_RDATA) :=
-       encode_word_Spec wks!"Address"
+        encode_nat_Spec 16 (length (wks!"Bit-Map"))
+  ThenC encode_word_Spec wks!"Address"
   ThenC encode_word_Spec wks!"Protocol"
   ThenC (encode_list_Spec encode_word_Spec wks!"Bit-Map")
   DoneC.
 
   Definition encode_HINFO_RDATA_Spec (hinfo : HINFO_RDATA) :=
-       encode_characterString_Spec hinfo!"CPU"
+       encode_unused_word_Spec 16 (* Unusued RDLENGTH Field *)
+  ThenC encode_characterString_Spec hinfo!"CPU"
   ThenC encode_characterString_Spec hinfo!"OS"
   DoneC.
 
   Definition encode_MX_RDATA_Spec (mx : MX_RDATA) :=
-       encode_word_Spec mx!"Preference"
+       encode_unused_word_Spec 16 (* Unusued RDLENGTH Field *)
+  ThenC encode_word_Spec mx!"Preference"
   ThenC encode_DomainName_Spec mx!"Exchange"
   DoneC.
 
   Definition encode_MINFO_RDATA_Spec (minfo : MINFO_RDATA) :=
-       encode_DomainName_Spec minfo!"rMailBx"
+       encode_unused_word_Spec 16 (* Unusued RDLENGTH Field *)
+  ThenC encode_DomainName_Spec minfo!"rMailBx"
   ThenC encode_DomainName_Spec minfo!"eMailBx"
   DoneC.
 
+  Definition encode_A_Spec (a : Memory.W) :=
+    encode_unused_word_Spec 16 (* Unused RDLENGTH Field *)
+    ThenC encode_word_Spec a
+    DoneC.
+
+  Definition encode_NS_Spec (domain : DomainName) :=
+    encode_unused_word_Spec 16 (* Unused RDLENGTH Field *)
+    ThenC encode_DomainName_Spec domain
+    DoneC.
+
+  Definition encode_CNAME_Spec (domain : DomainName) :=
+    encode_unused_word_Spec 16 (* Unused RDLENGTH Field *)
+    ThenC encode_DomainName_Spec domain
+    DoneC.
+
+    Definition encode_PTR_Spec (domain : DomainName) :=
+    encode_unused_word_Spec 16 (* Unused RDLENGTH Field *)
+    ThenC encode_DomainName_Spec domain
+    DoneC.
+
   Definition encode_rdata_Spec :=
   encode_SumType_Spec ResourceRecordTypeTypes
-  (icons encode_word_Spec (* A; host address 	[RFC1035] *)
-  (icons (encode_DomainName_Spec) (* NS; authoritative name server 	[RFC1035] *)
-  (icons (encode_DomainName_Spec)  (* CNAME; canonical name for an alias 	[RFC1035] *)
+  (icons encode_A_Spec (* A; host address 	[RFC1035] *)
+  (icons (encode_NS_Spec) (* NS; authoritative name server 	[RFC1035] *)
+  (icons (encode_CNAME_Spec)  (* CNAME; canonical name for an alias 	[RFC1035] *)
   (icons encode_SOA_RDATA_Spec  (* SOA rks the start of a zone of authority 	[RFC1035] *)
   (icons encode_WKS_RDATA_Spec (* WKS  well known service description 	[RFC1035] *)
-  (icons (encode_DomainName_Spec) (* PTR domain name pointer 	[RFC1035] *)
+  (icons (encode_PTR_Spec) (* PTR domain name pointer 	[RFC1035] *)
   (icons encode_HINFO_RDATA_Spec (* HINFO host information 	[RFC1035] *)
   (icons (encode_MINFO_RDATA_Spec) (* MINFO mailbox or mail list information 	[RFC1035] *)
   (icons encode_MX_RDATA_Spec  (* MX  mail exchange 	[RFC1035] *)
-  (icons encode_characterString_Spec inil)))))))))). (*TXT text strings 	[RFC1035] *)
+  (icons encode_TXT_Spec inil)))))))))). (*TXT text strings 	[RFC1035] *)
 
   Definition encode_resource_Spec(r : resourceRecord) :=
        encode_DomainName_Spec r!sNAME
   ThenC encode_enum_Spec RRecordType_Ws r!sTYPE
   ThenC encode_enum_Spec RRecordClass_Ws r!sCLASS
-  ThenC encode_word_Spec r!sTTL (* Missing length field*)
+  ThenC encode_word_Spec r!sTTL
   ThenC encode_rdata_Spec r!sRDATA
   DoneC.
 
@@ -136,15 +166,6 @@ Section DnsPacket.
   DoneC.
 
     Definition transformer : Transformer ByteString := ByteStringQueueTransformer.
-
-  Ltac normalize_compose :=
-    eapply encode_decode_correct_refineEquiv;
-    [ intros ? ?; symmetry;
-      repeat first [ etransitivity; [apply refineEquiv_compose_compose with (transformer := transformer)| ]
-                   | etransitivity; [apply refineEquiv_compose_Done with (transformer := transformer) | ]
-                   | apply refineEquiv_under_compose with (transformer := transformer) ];
-      intros; higher_order_reflexivity
-    | ].
 
   Lemma firstn_app {A}
     : forall (l1 l2 : list A),
@@ -197,6 +218,21 @@ Section DnsPacket.
     destruct l; simpl.
     intros; discriminate.
     intros; f_equal; eauto.
+  Qed.
+
+    Lemma firstn_skipn_self {A}
+      : forall (n m o : nat) (l l1 l2 l3 : list A),
+      (l1 ++ l2 ++ l3)%list = l ->
+      (|l1|) = n ->
+      (|l2|) = m ->
+      (|l3|) = o ->
+      l1 = firstn n l
+      /\ l2 = firstn m (skipn n l)
+      /\ l3 = firstn o (skipn (n + m) l).
+  Proof.
+    intros; subst; intuition;
+    eauto using firstn_skipn_app, skipn_app, firstn_app.
+    rewrite skipn_app; symmetry; apply firstn_app.
   Qed.
 
   Lemma length_firstn_skipn_app {A}
@@ -252,79 +288,6 @@ Section DnsPacket.
     rewrite (shatter_word_0 x0); reflexivity.
   Qed.
 
-  (*Ltac apply_compose :=
-    intros;
-    match goal with
-      H : cache_inv_Property ?P ?P_inv |- _ =>
-      first [eapply (compose_encode_correct_no_dep H); clear H
-            | eapply (compose_encode_correct H); clear H
-            ]
-    end. *)
-
-  (* Theorem characterString_decode_correct
-          {P : CacheDecode -> Prop}
-          (P_OK : cache_inv_Property P (fun P => forall (b : nat) cd, P cd -> P (addD cd b)))
-    : encode_decode_correct_f cache transformer (fun ls => lt (String.length ls) (pow2 8))
-                              encode_characterString_Spec
-                              (fun (bin' : _) (env : CacheDecode) =>
-                                 `(proj, rest, env') <- decode_nat 8 bin' env;
-                                   decode_string proj rest env')
-                              P.
-  Proof.
-    intros; normalize_compose.
-    eapply compose_encode_correct.
-    2: apply Nat_decode_correct.
-    2: eauto.
-    Focus 2.
-    unfold encode_decode_correct_f; intuition eauto.
-    eapply String_decode_correct; eauto.
-    eapply String_decode_correct in H3; intuition eauto.
-    eapply String_decode_correct in H3; intuition eauto.
-    destruct_ex; intuition; eexists _; eexists _; subst;
-      intuition eauto.
-    unfold cache_inv_Property in *; eauto.
-  Qed.
-*)
-
-  (*Ltac makeEvar T k :=
-    let x := fresh in evar (x : T); let y := eval unfold x in x in clear x; k y.
-
-  Ltac shelve_inv :=
-    let H' := fresh in
-    let data := fresh in
-    intros data H';
-    repeat destruct H';
-    match goal with
-    | H : ?P data |- ?P_inv' =>
-      is_evar P;
-      let P_inv' := (eval pattern data in P_inv') in
-      let P_inv := match P_inv' with ?P_inv data => P_inv end in
-      let new_P_T := type of P in
-      makeEvar new_P_T
-               ltac:(fun new_P =>
-                       unify P (fun data => new_P data /\ P_inv data)); apply (Logic.proj2 H)
-    end.
-
-  (* Commenting out until patched to work with wrinkles introduced by other examples. *)
-  (*Ltac solve_data_inv :=
-    first [ intros; exact I
-          | shelve_inv ].
-
-  Ltac build_decoder :=
-    first [ solve [eapply Enum_decode_correct; eauto ]
-          | solve [eapply Word_decode_correct ]
-
-          | solve [eapply Nat_decode_correct ]
-          | solve [eapply String_decode_correct ]
-          | solve [intros; eapply DomainName_decode_correct ]
-          | intros;
-            match goal with
-              |- encode_decode_correct_f
-                   _ _ _
-                   (encode_list_Spec _) _ _ =>
-              eapply FixList_decode_correct end
-          | apply_compose ]. *) *)
-
   Lemma decides_True' {A}
     : forall a, decides true ((fun _ : A => True) a).
   Proof.
@@ -377,6 +340,8 @@ Ltac decode_step :=
   | H : cache_inv_Property _ _
     |- appcontext [encode_decode_correct_f _ _ _ _ encode_word_Spec _ _] =>
     intros; revert H; eapply Word_decode_correct
+  | |- appcontext [encode_decode_correct_f _ _ _ _ (encode_unused_word_Spec' _ _) _ _] =>
+    apply unused_word_decode_correct
   | |- appcontext [encode_decode_correct_f _ _ _ _ encode_word_Spec _ _] =>
     eapply Word_decode_correct
   | |- appcontext [encode_decode_correct_f _ _ _ _ (encode_nat_Spec _) _ _] =>
@@ -423,26 +388,170 @@ Proof.
   simpl; intros; apply H; eauto.
 Qed.
 
+Lemma firstn_lt_decides {A}:
+  forall m n (l : list A),
+    (lt m n)%nat
+    -> decides true (lt (|firstn m l |) n)%nat.
+Proof.
+  simpl; intros; rewrite firstn_length.
+  eapply NPeano.Nat.min_lt_iff; eauto.
+Qed.
+
 Hint Resolve validDomainName_proj1_OK : decide_data_invariant_db.
 Hint Resolve validDomainName_proj2_OK : decide_data_invariant_db.
+Hint Resolve firstn_lt_decides : decide_data_invariant_db.
+
+Instance : DecideableEnsembles.Query_eq () :=
+  {| A_eq_dec a a' := match a, a' with (), () => left (eq_refl _) end |}.
+
+Definition resourceRecord_OK (rr : resourceRecord) :=
+SumType_index
+     ((Memory.W : Type)
+      :: DomainName
+         :: DomainName
+            :: SOA_RDATA
+               :: WKS_RDATA :: DomainName :: HINFO_RDATA :: MINFO_RDATA :: MX_RDATA :: [string : Type])
+     rr!sRDATA = rr!sTYPE /\
+   ith
+     (icons (B := fun T => T -> Prop) (fun _ : Memory.W => True)
+     (icons (B := fun T => T -> Prop) (fun a : DomainName => ValidDomainName a)
+     (icons (B := fun T => T -> Prop) (fun a : DomainName => ValidDomainName a)
+     (icons (B := fun T => T -> Prop) (fun a : SOA_RDATA =>
+               (True /\ ValidDomainName a!"contact_email") /\ ValidDomainName a!"sourcehost")
+     (icons (B := fun T => T -> Prop) (fun a : WKS_RDATA => True /\ (lt (|a!"Bit-Map" |)  (pow2 16)))
+     (icons (B := fun T => T -> Prop) (fun a : DomainName => ValidDomainName a)
+     (icons (B := fun T => T -> Prop) (fun a : HINFO_RDATA =>
+               (True /\ True /\ (lt (String.length a!"OS") (pow2 8))) /\
+               True /\ (lt (String.length a!"CPU") (pow2 8)))
+     (icons (B := fun T => T -> Prop) (fun a : MINFO_RDATA =>
+               (True /\ ValidDomainName a!"eMailBx") /\
+               ValidDomainName a!"rMailBx")
+     (icons (B := fun T => T -> Prop) (fun a : MX_RDATA => True /\ ValidDomainName a!"Exchange")
+     (icons (B := fun T => T -> Prop) (fun a : string =>
+               True /\ True /\ (lt (String.length a) (pow2 8))) inil))))))))))
+     (SumType_index
+        ((Memory.W : Type)
+         :: DomainName
+            :: DomainName
+               :: SOA_RDATA
+                  :: WKS_RDATA
+                     :: DomainName :: HINFO_RDATA :: MINFO_RDATA :: MX_RDATA :: [string : Type])
+        rr!sRDATA)
+     (SumType_proj
+        ((Memory.W : Type)
+         :: DomainName
+            :: DomainName
+               :: SOA_RDATA
+                  :: WKS_RDATA
+                     :: DomainName :: HINFO_RDATA :: MINFO_RDATA :: MX_RDATA :: [string : Type])
+        rr!sRDATA)
+/\ ValidDomainName rr!sNAME.
+
+Definition DNS_Packet_OK (data : packet) :=
+  lt (|data!"answers" |) (pow2 16)
+  /\ lt (|data!"authority" |) (pow2 16)
+  /\ lt (|data!"additional" |) (pow2 16)
+  /\ ValidDomainName (data!"question")!"qname"
+  /\ forall (rr : resourceRecord),
+      In rr (data!"answers" ++ data!"additional" ++ data!"authority")
+      -> resourceRecord_OK rr.
+
+    Definition GoodCache (env : CacheDecode) :=
+                     forall domain p,
+                     getD env p = Some domain
+                     -> ValidDomainName domain
+                        /\ (String.length domain > 0)%nat.
+
+    Lemma foo : forall (b : nat) (cd : CacheDecode), GoodCache cd -> GoodCache (addD cd b).
+    Admitted.
+
+    Lemma foo2
+      : forall cd p (b : nat) domain,
+        GoodCache cd
+        -> getD (addD cd b) p = Some domain
+        -> forall pre label post : string,
+            domain = (pre ++ label ++ post)%string ->
+            ValidLabel label -> (String.length label <= 63)%nat.
+    Admitted.
+
+    Lemma foo3
+      : forall cd p (b : nat) domain,
+        GoodCache cd
+        -> getD (addD cd b) p = Some domain
+        -> ValidDomainName domain.
+    Admitted.
+
+    Lemma foo4
+      : forall cd p (b : nat) domain,
+        GoodCache cd
+        -> getD (addD cd b) p = Some domain
+        -> gt (String.length domain) 0.
+    Admitted.
+
+    Lemma foo5
+      : forall cd p domain,
+        GoodCache cd
+        -> getD cd p = Some domain
+        -> ValidDomainName domain.
+    Admitted.
+
+    Lemma foo6
+      : forall cd p domain,
+        GoodCache cd
+        -> getD cd p = Some domain
+        -> gt (String.length domain) 0.
+    Admitted.
+
+    Lemma foo7
+      : forall cd p domain,
+        GoodCache cd
+        -> getD cd p = Some domain
+        -> forall pre label post : string,
+            domain = (pre ++ label ++ post)%string ->
+            ValidLabel label -> (String.length label <= 63)%nat.
+    Admitted.
+
+    Lemma foo8
+      : forall cd p p0 domain domain',
+        GoodCache cd
+        -> ValidDomainName domain' /\ (String.length domain' > 0)%nat
+        -> getD (addD cd (domain', p0)) p = Some domain
+        -> forall pre label post : string,
+            domain = (pre ++ label ++ post)%string ->
+            ValidLabel label -> (String.length label <= 63)%nat.
+    Admitted.
+
+    Lemma foo9
+      : forall cd p p0 domain domain',
+        GoodCache cd
+        -> ValidDomainName domain' /\ (String.length domain' > 0)%nat
+        -> getD (addD cd (domain', p0)) p = Some domain
+        -> ValidDomainName domain.
+    Admitted.
+
+    Lemma foo10
+      : forall cd p p0 domain domain',
+        GoodCache cd
+        -> ValidDomainName domain' /\ (String.length domain' > 0)%nat
+        -> getD (addD cd (domain', p0)) p = Some domain
+        -> gt (String.length domain) 0.
+    Admitted.
+
+    Lemma foo11
+      : forall (ce : CacheEncode) (l : DomainName) (p1 p2 : word 8),
+        getE ce l = Some (p1, p2) -> wlt (natToWord 8 191) p1.
+    Admitted.
+
 
 Definition packet_decoder
-             pred
     : { decodePlusCacheInv |
         exists P_inv,
         (cache_inv_Property (snd decodePlusCacheInv) P_inv
-        -> encode_decode_correct_f _ transformer pred (fun _ _ => True) encode_packet_Spec (fst decodePlusCacheInv) (snd decodePlusCacheInv))
+        -> encode_decode_correct_f _ transformer DNS_Packet_OK (fun _ _ => True) encode_packet_Spec (fst decodePlusCacheInv) (snd decodePlusCacheInv))
         /\ cache_inv_Property (snd decodePlusCacheInv) P_inv}.
   Proof.
     start_synthesizing_decoder.
-    pose_string_ids.
-    intros; eapply encode_decode_correct_refineEquiv;
-      [intros ? ?; symmetry;
-       repeat first [ etransitivity; [apply refineEquiv_compose_compose with (transformer := transformer)| ]
-                    | etransitivity; [apply refineEquiv_compose_Done with (transformer := transformer) | ]
-                    | apply refineEquiv_under_compose with (transformer := transformer) ];
-       intros; higher_order_reflexivity
-      | pose_string_ids ].
+    normalize_compose transformer.
     decode_step.
     decode_step.
     decode_step.
@@ -487,28 +596,16 @@ Definition packet_decoder
     decode_step.
     decode_step.
     decode_step.
-    simpl.
-    admit. (* Need constraint on the number of answers: *)
-    (* ((|data!StringId8 |) < pow2 16) *)
     decode_step.
     decode_step.
     decode_step.
-    admit. (* Need constraint on the number of authority responses. *)
-    (* ((|data!StringId8 |) < pow2 16) *)
     decode_step.
     decode_step.
     decode_step.
-    admit. (* Need constraint on the number of additional responses. *)
-    (* ((|data!StringId10 |) < pow2 16) *)
     decode_step.
     decode_step.
     decode_step.
-    simpl.
-    (* Need constraint on the validity of domainNames in question*)
-    (* ValidDomainName (data!"question")!"qname" *)
-    admit.
     decode_step.
-    apply_compose.
     decode_step.
     decode_step.
     decode_step.
@@ -520,7 +617,17 @@ Definition packet_decoder
     decode_step.
     decode_step.
     decode_step.
-    decode_step. (* intros; eapply FixList_decode_correct. *)
+    decode_step.
+    decode_step.
+    decode_step.
+    decode_step.
+    decode_step.
+    decode_step.
+    intros; instantiate (1 := fun _ _ => True).
+    decode_step.
+    decode_step.
+    decode_step.
+    decode_step.
     decode_step.
     decode_step.
     decode_step.
@@ -540,6 +647,7 @@ Definition packet_decoder
     decode_step.
     decode_step.
     eapply SumType_decode_correct with
+    (idx := proj12)
     (encoders := (icons _
            (icons _
               (icons _
@@ -588,32 +696,44 @@ Definition packet_decoder
     intro; pattern idx.
     eapply Iterate_Ensemble_equiv' with (idx := idx); simpl.
     apply Build_prim_and.
+    unfold encode_A_Spec, encode_unused_word_Spec.
     repeat decode_step.
     apply Build_prim_and.
+    unfold encode_NS_Spec, encode_unused_word_Spec.
     repeat decode_step.
     apply Build_prim_and.
+    unfold encode_CNAME_Spec, encode_unused_word_Spec.
     repeat decode_step.
     apply Build_prim_and.
-    repeat decode_step.
-    (* Another constraint on data  intros; clear; admit. *)
-    apply Build_prim_and.
-    decode_step.
-    decode_step.
-    decode_step.
-    decode_step.
-    decode_step.
-    decode_step.
-    decode_step.
-    decode_step.
-    decode_step.
-    decode_step.
-    decode_step.
-    decode_step.
-    decode_step.
+    unfold encode_SOA_RDATA_Spec, encode_unused_word_Spec.
     repeat decode_step.
     apply Build_prim_and.
+    decode_step.
+    decode_step.
+    decode_step.
+    decode_step.
+    decode_step.
+    decode_step.
+    decode_step.
+    decode_step.
+    decode_step.
+    decode_step.
+    decode_step.
+    decode_step.
+    decode_step.
+    repeat decode_step.
+    repeat decode_step.
+    repeat decode_step.
     repeat decode_step.
     apply Build_prim_and.
+    unfold encode_PTR_Spec, encode_unused_word_Spec.
+    repeat decode_step.
+    apply Build_prim_and.
+    unfold encode_HINFO_RDATA_Spec, encode_unused_word_Spec.
+    decode_step.
+    decode_step.
+    decode_step.
+    decode_step.
     decode_step.
     decode_step.
     decode_step.
@@ -646,10 +766,18 @@ Definition packet_decoder
     decode_step.
     decode_step.
     apply Build_prim_and.
+    unfold encode_MINFO_RDATA_Spec, encode_unused_word_Spec.
     repeat decode_step.
     apply Build_prim_and.
+    unfold encode_MX_RDATA_Spec, encode_unused_word_Spec.
     repeat decode_step.
     apply Build_prim_and.
+    unfold encode_TXT_Spec, encode_unused_word_Spec.
+    decode_step.
+    decode_step.
+    decode_step.
+    decode_step.
+    decode_step.
     decode_step.
     decode_step.
     decode_step.
@@ -660,541 +788,683 @@ Definition packet_decoder
     decode_step.
     decode_step.
     decode_step.
-    decode_step.
+    (* Need an invariant on the resource records in response. *)
+    intros; clear.
+    simpl.
     repeat instantiate (1 := fun _ _ => True).
-    intros; clear; admit.
+    simpl; eauto.
+    decode_step.
+    decode_step.
+    intros.
+    destruct H17 as [ [ [ [ [? ?] ? ] ? ] ? ] ?].
+    subst proj12.
+    pattern data.
+    apply H17.
+
+    repeat instantiate (1 := fun _ _ => True).
+    intros.
+    let a'' := fresh in
+    rename a' into a'';
+      repeat destruct a'' as [ ? | a''] ; auto.
     decode_step.
     split; intros.
     intuition.
     rewrite !app_length.
-    rewrite H20, H21, H22.
+    rewrite H16, H17, H18.
     reflexivity.
     intuition; intros.
-    Focus 2.
-    Show Existentials.
-
-
-    intros; simpl.
-    4: decode_step.
-    2: decode_step.
-
-    simpl.
-
-
-
-
-
-    repeat decode_step.
-
+    apply H31; eauto.
+    apply H31; eauto.
+    apply H31; eauto.
     decode_step.
-    decode_step.
-    decode_step.
-    decode_step.
-    eapply String_decode_correct.
-    decode_step.
-    decode_step.
-    intros; eapply encode_decode_correct_finish.
-    build_fully_determined_type.
-    decide_data_invariant.
-    decode_step.
-    intros; instantiate (1 := fun _ _ => True).
-    decode_step.
-    decode_step.
-    decode_step.
-    decode_step.
-    decode_step.
-    decode_step.
-    decode_step.
-    eapply String_decode_correct.
-    decode_step.
-    decode_step.
-    intros; eapply encode_decode_correct_finish.
-    build_fully_determined_type.
-    decide_data_invariant.
-    decode_step.
-    intros; instantiate (1 := fun _ _ => True).
-    decode_step.
-    decode_step.
-
-
-    intros; instantiate (1 := fun _ _ => True).
-
-    solve_data_inv.
-let H' := fresh in
-  let data := fresh in
-  intros data H';
-  repeat destruct H';
-  match goal with
-  | H : ?P data |- ?P_inv' =>
-    is_evar P;
-    let P_inv' := (eval pattern data in P_inv') in
-    let P_inv := match P_inv' with ?P_inv data => P_inv end in
-    let new_P_T := type of P in
-    makeEvar new_P_T
-             ltac:(fun new_P =>
-                     unify P (fun data => new_P data /\ P_inv data)); apply (Logic.proj2 H)
-  end.
-
-    shelve_inv.
-
-    build_fully_determined_type.
-    unfold GetAttribute, GetAttributeRaw in *;
-      simpl in *; intros; intuition.
-    subst.
-    repeat
-        first [ eapply decides_and
-          | eapply decides_assumption; eassumption
-          | apply decides_eq_refl
-          | solve [eauto with decide_data_invariant_db]
-          | eapply decides_dec_eq; auto using Peano_dec.eq_nat_dec, weq ].
-    first [ eapply decides_and
-          | eapply decides_assumption; eassumption
-          | apply decides_eq_refl
-          | solve [eauto with decide_data_invariant_db]
-          | eapply decides_dec_eq; auto using Peano_dec.eq_nat_dec, weq ].
-        first [ eapply decides_and
-          | eapply decides_assumption; eassumption
-          | solve [eauto with decide_data_invariant_db]
-          | eapply decides_dec_eq; auto using Peano_dec.eq_nat_dec, weq ].
-                first [ eapply decides_and
-          | eapply decides_assumption; eassumption
-          | apply decides_eq_refl
-          | solve [eauto with decide_data_invariant_db]
-          | eapply decides_dec_eq; auto using Peano_dec.eq_nat_dec, weq ].
-        first [ eapply decides_and
-          | eapply decides_assumption; eassumption
-          | apply decides_eq_refl
-          | solve [eauto with decide_data_invariant_db]
-          | eapply decides_dec_eq; auto using Peano_dec.eq_nat_dec, weq ].
-        first [ eapply decides_and
-          | eapply decides_assumption; eassumption
-          | apply decides_eq_refl
-          | solve [eauto with decide_data_invariant_db]
-          | eapply decides_dec_eq; auto using Peano_dec.eq_nat_dec, weq ].
-        eapply decides_eq_refl.
-        eapply decides_eq_refl.
-        eapply decides_eq_refl.
-    eapply decides_and
-    decode_step.
-
-
-    apply Build_prim_and.
-    repeat decode_step.
-
-
-  (* Processes the goal by either: *)
-  match goal with
-  (* A) decomposing one of the parser combinators, *)
-  | |- _ => apply_compose
-  (* B) applying one of the rules for a base type  *)
-  | H : cache_inv_Property _ _
-    |- appcontext [encode_decode_correct_f _ _ _ _ encode_word_Spec _ _] =>
-    intros; revert H; eapply Word_decode_correct
-  | |- appcontext [encode_decode_correct_f _ _ _ _ encode_word_Spec _ _] =>
-    eapply Word_decode_correct
-  | |- appcontext [encode_list_Spec] =>
-    intros; eapply FixList_decode_correct
-  | |- appcontext [encode_decode_correct_f _ _ _ _ (encode_nat_Spec _) _ _] =>
-    eapply Nat_decode_correct
-  | |- appcontext [encode_decode_correct_f _ _ _ _ (encode_enum_Spec _) _ _] =>
-    eapply Enum_decode_correct
-  (* C) Discharging a side condition of one of the base rules *)
-  | |- NoDupVector _ => Discharge_NoDupVector
-    intros; apply Vector_predicate_rest_True
-  | _ => solve [solve_data_inv]
-  (* D) Solving the goal once all the byte string has been parsed *)
-  | _ =>  solve [simpl; intros;
-                 eapply encode_decode_correct_finish;
-                 [ build_fully_determined_type
-                 | decide_data_invariant ] ]
-  end.
-
-    decode_step.
-
-
-    apply Build_prim_and.
-    repeat decode_step.
-
-
-
-
-    build_decoder.
-    apply Build_prim_and.
-    build_decoder.
-    apply Build_prim_and.
-    {
-      build_decoder.
-      build_decoder.
-      solve_data_inv.
-      build_decoder.
-      build_decoder.
-      solve_data_inv.
-      build_decoder.
-      build_decoder.
-      solve_data_inv.
-      build_decoder.
-      build_decoder.
-      solve_data_inv.
-      build_decoder.
-      build_decoder.
-      solve_data_inv.
-      build_decoder.
-      build_decoder.
-      solve_data_inv.
-      build_decoder.
-      build_decoder.
-      solve_data_inv.
-      unfold encode_decode_correct_f; intuition eauto.
-      destruct data as [? [? [? [? [? [? [? [ ] ] ] ] ] ] ] ].
-      unfold GetAttribute, GetAttributeRaw in *.
-      subst; simpl.
-      computes_to_inv; injections.
-      eexists; intuition eauto; simpl.
-      match goal with
-        |- ?f ?a ?b ?c = ?P =>
-        let P' := (eval pattern a, b, c in P) in
-        let f' := match P' with ?f a b c => f end in
-      unify f f'; reflexivity
-      end.
-      injections; eauto.
-      eexists _; eexists _.
-    intuition eauto.
-    injections; eauto.
-    injections.
-    solve_predicate.
-    injections; eauto.
-    injections; eauto.
-    injections; eauto.
-    injections; eauto.
-    injections; eauto.
-    injections; eauto.
-    injections; eauto.
-    injections; eauto.
-    injections; eauto.
-    injections; eauto.
-    injections; eauto.
-    injections; eauto.
-    }
-    apply Build_prim_and.
-    {
-      build_decoder.
-      build_decoder.
-      solve_data_inv.
-      build_decoder.
-      build_decoder.
-      solve_data_inv.
-      build_decoder.
-      build_decoder.
-      revert H21; build_decoder.
-      shelve_inv.
-      unfold encode_decode_correct_f; intuition eauto.
-      destruct data as [? [? [? [ ] ] ] ].
-      unfold GetAttribute, GetAttributeRaw in *.
-      subst; simpl.
-      computes_to_inv; injections.
-      eexists; intuition eauto; simpl.
-      match goal with
-        |- ?f ?a ?b ?c = ?P =>
-        let P' := (eval pattern a, b, c in P) in
-        let f' := match P' with ?f a b c => f end in
-        unify f f'; reflexivity
-      end.
-      simpl in H25; injections; eauto.
-      eexists _; eexists _.
-      intuition eauto.
-      injections; eauto.
-      injections.
-      solve_predicate.
-      injections; eauto.
-      injections; eauto.
-      injections; eauto.
-      injections; eauto.
-      injections; eauto.
-    }
-    apply Build_prim_and.
-    build_decoder.
-    apply Build_prim_and.
-    {
-      build_decoder.
-      build_decoder.
-      solve_data_inv.
-      build_decoder.
-      build_decoder.
-      solve_data_inv.
-      unfold encode_decode_correct_f; intuition eauto.
-      destruct data as [? [? [ ] ] ].
-      unfold GetAttribute, GetAttributeRaw in *.
-      subst; simpl.
-      computes_to_inv; injections.
-      eexists; intuition eauto; simpl.
-      match goal with
-        |- ?f ?a ?b ?c = ?P =>
-        let P' := (eval pattern a, b, c in P) in
-        let f' := match P' with ?f a b c => f end in
-        unify f f'; reflexivity
-      end.
-      injections; eauto.
-      eexists _; eexists _.
-      intuition eauto.
-      injections; eauto.
-      injections; solve_predicate.
-      injections; eauto.
-      injections; eauto.
-      injections; eauto.
-      injections; eauto.
-      injections; solve_predicate.
-    }
-    apply Build_prim_and.
-    { build_decoder.
-      build_decoder.
-      solve_data_inv.
-      build_decoder.
-      build_decoder.
-      solve_data_inv.
-      unfold encode_decode_correct_f; intuition eauto.
-      destruct data as [? [? [ ] ] ].
-      unfold GetAttribute, GetAttributeRaw in *.
-      subst; simpl.
-      computes_to_inv; injections.
-      eexists; intuition eauto; simpl.
-      match goal with
-        |- ?f ?a ?b ?c = ?P =>
-        let P' := (eval pattern a, b, c in P) in
-        let f' := match P' with ?f a b c => f end in
-        unify f f'; reflexivity
-      end.
-      injections; eauto.
-      eexists _; eexists _.
-      intuition eauto.
-      injections; eauto.
-      injections; solve_predicate.
-      injections; eauto.
-      injections; eauto.
-      injections; eauto.
-      injections; eauto.
-      injections; solve_predicate.
-      injections; solve_predicate.
-      injections; solve_predicate.
-    }
-    apply Build_prim_and.
-    { build_decoder.
-      build_decoder.
-      solve_data_inv.
-      build_decoder.
-      build_decoder.
-      solve_data_inv.
-      unfold encode_decode_correct_f; intuition eauto.
-      destruct data as [? [? [ ] ] ].
-      unfold GetAttribute, GetAttributeRaw in *.
-      subst; simpl.
-      computes_to_inv; injections.
-      eexists; intuition eauto; simpl.
-      match goal with
-        |- ?f ?a ?b ?c = ?P =>
-        let P' := (eval pattern a, b, c in P) in
-        let f' := match P' with ?f a b c => f end in
-        unify f f'; reflexivity
-      end.
-      injections; eauto.
-      eexists _; eexists _.
-      intuition eauto.
-      injections; eauto.
-      injections; solve_predicate.
-      injections; eauto.
-      injections; eauto.
-      injections; eauto.
-      injections; eauto.
-      injections; solve_predicate.
-    }
-    apply Build_prim_and.
-    build_decoder.
-    eauto.
-    shelve_inv.
-    { unfold encode_decode_correct_f; intuition eauto.
-      destruct data as [? [? [? [? [? [ ] ] ] ] ] ].
-      unfold GetAttribute, GetAttributeRaw in *.
-      simpl in *; subst.
-      computes_to_inv; injections.
-      eexists; intuition eauto; simpl.
-      match goal with
-      |- ?f ?a ?b ?c = ?P =>
-      let P' := (eval pattern a, b, c in P) in
-      let f' := match P' with ?f a b c => f end in
-      unify f f'; reflexivity
-      end.
-      injections; eauto.
-      eexists _; eexists _.
-      intuition eauto.
-      injections; eauto.
-      solve_predicate.
-      injections; eauto.
-      injections; eauto.
-      injections; eauto.
-      injections; eauto.
-      injections; eauto.
-      injections; eauto.
-      injections; eauto.
-      injections; eauto.
-      injections; eauto.
-      injections; eauto.
-    }
-    simpl; intros; intuition eauto.
-    rewrite !app_length, H20, H21, H22.
-    reflexivity.
-    generalize data H15 x H34.
-    shelve_inv.
-    generalize data H15 x H34.
-    shelve_inv.
-    generalize data H15 x H34.
-    shelve_inv.
-    generalize data H15 x H34.
-    shelve_inv.
-    simpl; intros; intuition eauto.
-    unfold encode_decode_correct_f; intuition eauto.
-    repeat destruct data.
-    repeat destruct prim_snd.
-    unfold GetAttribute, GetAttributeRaw in *.
-    computes_to_inv.
-    repeat match goal with
-             H : context [ilist2.ith2]
-             |- _ => simpl in H
-           end.
-    repeat match goal with
-             H : ?Z
-             |- _ => match Z with context [ilist2.ith2 _ _] => simpl in H
-                     end
-           end.
-    simpl.
-    destruct prim_fst7.
-    destruct prim_snd.
-    simpl in H21; simpl in H22; simpl in H23.
-    destruct prim_snd.
-    simpl in H21.
-    destruct prim_snd.
-    simpl.
-    eexists; repeat split.
+    simpl; intros;
+      eapply encode_decode_correct_finish.
+    let a' := fresh in
+  intros a'; repeat destruct a' as [? a'];
+  (* Show that it is determined by the constraints (equalities) *)
+  (* inferred during parsing. *)
+  unfold GetAttribute, GetAttributeRaw in *;
+  simpl in *; intros;
+  (* Decompose data predicate *) intuition.
+    eapply firstn_skipn_self in H19; try eassumption.
+    intuition.
+    clear H21 H22 H23.
+  (* Substitute any inferred equalities *)
     repeat match goal with
              H : WS _ WO = _ |- _ =>
-             let H' := fresh in
-             pose proof (f_equal (@whd _) H) as H'; simpl in H';
-               rewrite H'; clear H' H
+             apply (f_equal (@whd 0)) in H;
+               simpl in H; rewrite H in *; clear H
            end.
-    simpl in *.
-    revert H29 H27 H28; subst.
-    injection H21; intros ? ?; subst.
-    instantiate (2 := fun al ext env' =>
-                         Some
-                           ({|
-      ilist.prim_fst := _;
-      ilist.prim_snd := {|
-                         ilist.prim_fst := _;
-                        ilist.prim_snd := {|
-                                          ilist.prim_fst := _;
-                                          ilist.prim_snd := {|
-                                                  ilist.prim_fst := _;
-                                                  ilist.prim_snd := {|
-                                                  ilist.prim_fst := _;
-                                                  ilist.prim_snd := {|
-                                                  ilist.prim_fst := _;
-                                                  ilist.prim_snd := {|
-                                                  ilist.prim_fst := _;
-                                                  ilist.prim_snd := {|
-                                                  ilist.prim_fst := _;
-                                                  ilist.prim_snd := {|
-                                                  ilist.prim_fst := {|
-                                                  ilist.prim_fst := _;
-                                                  ilist.prim_snd := {|
-                                                  ilist.prim_fst := _;
-                                                  ilist.prim_snd := {|
-                                                  ilist.prim_fst := _;
-                                                  ilist.prim_snd := () |} |} |};
-                                                  ilist.prim_snd := {|
-                                                  ilist.prim_fst := firstn proj7 al;
-                                                  ilist.prim_snd := {|
-                                                  ilist.prim_fst := firstn proj8 (skipn (proj7 + proj9) al);
-                                                  ilist.prim_snd := {|
-                                                  ilist.prim_fst := firstn proj9 (skipn proj7 al); ilist.prim_snd := () |}
-                                                   |} |} |} |} |} |} |} |} |} |} |},
-     ext, env')).
-    simpl; intros; repeat progress f_equal.
-    eauto.
-    eauto.
-    eauto.
-    subst; apply firstn_app.
-    subst; apply firstn_skipn_app.
-    subst; rewrite skipn_app.
-    apply firstn_app.
-    injections; eauto.
-    injections; eauto.
-    eexists _; eexists _; split; split; eauto.
-    injections; simpl; eauto.
-    split.
-    simpl in H21.
-    injection H21; intros; subst.
-    unfold GetAttribute, GetAttributeRaw; simpl.
+    let a' := fresh in
+    rename prim_fst7 into a'; repeat destruct a' as [? a'];
+      simpl in *.
+    subst.
+  (* And unify with original object *) reflexivity.
+    decide_data_invariant.
+    instantiate (1 := true).
+    simpl; intros.
+    rewrite firstn_skipn_self' in H13.
+    apply H17 in H13.
+    unfold resourceRecord_OK; simpl.
     intuition eauto.
-    solve_predicate.
-    injections; eauto.
-    eapply H18.
-    rewrite firstn_skipn_self' in H34.
-    eauto.
-    eauto.
-    rewrite H17; clear; omega.
-    eapply H18.
-    rewrite firstn_skipn_self' in H34.
-    eauto.
-    rewrite H17; clear; omega.
-    eapply H18.
-    rewrite firstn_skipn_self' in H34.
-    eauto.
-    rewrite H17; clear; omega.
-    eapply H18.
-    rewrite firstn_skipn_self' in H34.
-    eauto.
-    rewrite H17; clear; omega.
-    revert H17 H11; clear.
-    rewrite Plus.plus_assoc; intros.
-    erewrite length_firstn_skipn_app by eauto.
-    apply H11.
-    revert H17 H10; clear.
-    rewrite Plus.plus_assoc; intros.
-    erewrite length_firstn_skipn_app' by eauto.
-    apply H10.
-    revert H17 H9; clear.
-    rewrite Plus.plus_assoc; intros.
-    erewrite length_firstn_skipn_app'' by eauto.
-    apply H9.
-    apply whd_word_1_refl.
-    apply whd_word_1_refl.
-    apply whd_word_1_refl.
-    apply whd_word_1_refl.
-    apply whd_word_1_refl.
-    revert H17; clear.
-    rewrite Plus.plus_assoc; intros.
-    eapply length_firstn_skipn_app''; eauto.
-    revert H17; clear.
-    rewrite Plus.plus_assoc; intros.
-    eapply length_firstn_skipn_app'; eauto.
-    revert H17; clear.
-    rewrite Plus.plus_assoc; intros.
-    eapply length_firstn_skipn_app; eauto.
-    eapply firstn_skipn_self'.
-    rewrite H17; omega.
-    simpl in H21.
-    injection H21; intros; subst.
-    eauto.
-    repeat instantiate (1 := fun _ => True); admit.
+    omega.
+
+    instantiate (17 := GoodCache).
+    unfold cache_inv_Property; repeat split;
+      eauto using foo, foo2, foo4, foo6, foo7, foo8, foo10, foo11;
+      try solve [ eapply foo3 in H1; intuition eauto ];
+      try solve [ eapply foo9 in H2; intuition eauto ];
+      try solve [ eapply foo5 in H1; intuition eauto ].
+    instantiate (1 := fun _ => True); exact I.
+    intro; pattern idx.
+    eapply Iterate_Ensemble_equiv' with (idx := idx); simpl.
+    apply Build_prim_and.
+    unfold cache_inv_Property; repeat split;
+      eauto using foo, foo2, foo4, foo6, foo7, foo8, foo10, foo11;
+      try solve [ eapply foo3 in H1; intuition eauto ];
+      try solve [ eapply foo9 in H2; intuition eauto ];
+      try solve [ eapply foo5 in H1; intuition eauto ].
+    instantiate (1 := fun _ => True); exact I.
+    apply Build_prim_and.
+    unfold cache_inv_Property; repeat split;
+      eauto using foo, foo2, foo4, foo6, foo7, foo8, foo10, foo11;
+      try solve [ eapply foo3 in H1; intuition eauto ];
+      try solve [ eapply foo9 in H2; intuition eauto ];
+      try solve [ eapply foo5 in H1; intuition eauto ];
+      try solve [instantiate (1 := fun _ => True); exact I].
+    apply Build_prim_and.
+    unfold cache_inv_Property; repeat split;
+      eauto using foo, foo2, foo4, foo6, foo7, foo8, foo10, foo11;
+      try solve [ eapply foo3 in H1; intuition eauto ];
+      try solve [ eapply foo9 in H2; intuition eauto ];
+      try solve [ eapply foo5 in H1; intuition eauto ].
+    instantiate (1 := fun _ => True); exact I.
+    apply Build_prim_and.
+    unfold cache_inv_Property; repeat split;
+      eauto using foo, foo2, foo4, foo6, foo7, foo8, foo10, foo11;
+      try solve [ eapply foo3 in H1; intuition eauto ];
+      try solve [ eapply foo9 in H2; intuition eauto ];
+      try solve [ eapply foo5 in H1; intuition eauto ];
+      try solve [instantiate (1 := fun _ => True); exact I].
+    apply Build_prim_and.
+    unfold cache_inv_Property; repeat split;
+      eauto using foo, foo2, foo4, foo6, foo7, foo8, foo10, foo11;
+      try solve [ eapply foo3 in H1; intuition eauto ];
+      try solve [ eapply foo9 in H2; intuition eauto ];
+      try solve [ eapply foo5 in H1; intuition eauto ].
+    instantiate (1 := fun _ => True); exact I.
+    apply Build_prim_and.
+    unfold cache_inv_Property; repeat split;
+      eauto using foo, foo2, foo4, foo6, foo7, foo8, foo10, foo11;
+      try solve [ eapply foo3 in H1; intuition eauto ];
+      try solve [ eapply foo9 in H2; intuition eauto ];
+      try solve [ eapply foo5 in H1; intuition eauto ];
+      try solve [instantiate (1 := fun _ => True); exact I].
+    apply Build_prim_and.
+    unfold cache_inv_Property; repeat split;
+      eauto using foo, foo2, foo4, foo6, foo7, foo8, foo10, foo11;
+      try solve [ eapply foo3 in H1; intuition eauto ];
+      try solve [ eapply foo9 in H2; intuition eauto ];
+      try solve [ eapply foo5 in H1; intuition eauto ];
+      try solve [instantiate (1 := fun _ => True); exact I].
+    apply Build_prim_and.
+    unfold cache_inv_Property; repeat split;
+      eauto using foo, foo2, foo4, foo6, foo7, foo8, foo10, foo11;
+      try solve [ eapply foo3 in H1; intuition eauto ];
+      try solve [ eapply foo9 in H2; intuition eauto ];
+      try solve [ eapply foo5 in H1; intuition eauto ];
+      try solve [instantiate (1 := fun _ => True); exact I].
+    apply Build_prim_and.
+    unfold cache_inv_Property; repeat split;
+      eauto using foo, foo2, foo4, foo6, foo7, foo8, foo10, foo11;
+      try solve [ eapply foo3 in H1; intuition eauto ];
+      try solve [ eapply foo9 in H2; intuition eauto ];
+      try solve [ eapply foo5 in H1; intuition eauto ];
+      try solve [instantiate (1 := fun _ => True); exact I].
+    apply Build_prim_and.
+    unfold cache_inv_Property; repeat split;
+      eauto using foo, foo2, foo4, foo6, foo7, foo8, foo10, foo11;
+      try solve [ eapply foo3 in H1; intuition eauto ];
+      try solve [ eapply foo9 in H2; intuition eauto ];
+      try solve [ eapply foo5 in H1; intuition eauto ];
+      try solve [instantiate (1 := fun _ => True); exact I].
+    exact I.
+    try solve [instantiate (1 := fun _ => True); exact I].
+    try solve [instantiate (1 := fun _ => True); exact I].
     Grab Existential Variables.
-    exact 0. (* Length of the Bit-Map in WKS RDATA. *)
-    apply (@Fin.F1 _). (* RDATA Type. *)
+    admit.
     apply Peano_dec.eq_nat_dec.
-    intros; destruct (weqb a a') eqn:Heq; [left | right].
-    apply weqb_sound; eauto.
-    intro; apply weqb_true_iff in H; congruence.
+    apply Peano_dec.eq_nat_dec.
+    apply Peano_dec.eq_nat_dec.
+    apply weq.
+    apply weq.
+    apply weq.
+    apply weq.
+    apply weq.
+    (* Still need decideable equality lemmas for: lists of resource *)
   Defined.
 
   Definition packetDecoderImpl := Eval simpl in (projT1 packet_decoder).
 
-  Print packetDecoderImpl. *)
+  Print packetDecoderImpl.
+
+  (*     intros; simpl. *)
+(*     4: decode_step. *)
+(*     2: decode_step. *)
+
+(*     simpl. *)
+
+
+
+
+
+(*     repeat decode_step. *)
+
+(*     decode_step. *)
+(*     decode_step. *)
+(*     decode_step. *)
+(*     decode_step. *)
+(*     eapply String_decode_correct. *)
+(*     decode_step. *)
+(*     decode_step. *)
+(*     intros; eapply encode_decode_correct_finish. *)
+(*     build_fully_determined_type. *)
+(*     decide_data_invariant. *)
+(*     decode_step. *)
+(*     intros; instantiate (1 := fun _ _ => True). *)
+(*     decode_step. *)
+(*     decode_step. *)
+(*     decode_step. *)
+(*     decode_step. *)
+(*     decode_step. *)
+(*     decode_step. *)
+(*     decode_step. *)
+(*     eapply String_decode_correct. *)
+(*     decode_step. *)
+(*     decode_step. *)
+(*     intros; eapply encode_decode_correct_finish. *)
+(*     build_fully_determined_type. *)
+(*     decide_data_invariant. *)
+(*     decode_step. *)
+(*     intros; instantiate (1 := fun _ _ => True). *)
+(*     decode_step. *)
+(*     decode_step. *)
+
+
+(*     intros; instantiate (1 := fun _ _ => True). *)
+
+(*     solve_data_inv. *)
+(* let H' := fresh in *)
+(*   let data := fresh in *)
+(*   intros data H'; *)
+(*   repeat destruct H'; *)
+(*   match goal with *)
+(*   | H : ?P data |- ?P_inv' => *)
+(*     is_evar P; *)
+(*     let P_inv' := (eval pattern data in P_inv') in *)
+(*     let P_inv := match P_inv' with ?P_inv data => P_inv end in *)
+(*     let new_P_T := type of P in *)
+(*     makeEvar new_P_T *)
+(*              ltac:(fun new_P => *)
+(*                      unify P (fun data => new_P data /\ P_inv data)); apply (Logic.proj2 H) *)
+(*   end. *)
+
+(*     shelve_inv. *)
+
+(*     build_fully_determined_type. *)
+(*     unfold GetAttribute, GetAttributeRaw in *; *)
+(*       simpl in *; intros; intuition. *)
+(*     subst. *)
+(*     repeat *)
+(*         first [ eapply decides_and *)
+(*           | eapply decides_assumption; eassumption *)
+(*           | apply decides_eq_refl *)
+(*           | solve [eauto with decide_data_invariant_db] *)
+(*           | eapply decides_dec_eq; auto using Peano_dec.eq_nat_dec, weq ]. *)
+(*     first [ eapply decides_and *)
+(*           | eapply decides_assumption; eassumption *)
+(*           | apply decides_eq_refl *)
+(*           | solve [eauto with decide_data_invariant_db] *)
+(*           | eapply decides_dec_eq; auto using Peano_dec.eq_nat_dec, weq ]. *)
+(*         first [ eapply decides_and *)
+(*           | eapply decides_assumption; eassumption *)
+(*           | solve [eauto with decide_data_invariant_db] *)
+(*           | eapply decides_dec_eq; auto using Peano_dec.eq_nat_dec, weq ]. *)
+(*                 first [ eapply decides_and *)
+(*           | eapply decides_assumption; eassumption *)
+(*           | apply decides_eq_refl *)
+(*           | solve [eauto with decide_data_invariant_db] *)
+(*           | eapply decides_dec_eq; auto using Peano_dec.eq_nat_dec, weq ]. *)
+(*         first [ eapply decides_and *)
+(*           | eapply decides_assumption; eassumption *)
+(*           | apply decides_eq_refl *)
+(*           | solve [eauto with decide_data_invariant_db] *)
+(*           | eapply decides_dec_eq; auto using Peano_dec.eq_nat_dec, weq ]. *)
+(*         first [ eapply decides_and *)
+(*           | eapply decides_assumption; eassumption *)
+(*           | apply decides_eq_refl *)
+(*           | solve [eauto with decide_data_invariant_db] *)
+(*           | eapply decides_dec_eq; auto using Peano_dec.eq_nat_dec, weq ]. *)
+(*         eapply decides_eq_refl. *)
+(*         eapply decides_eq_refl. *)
+(*         eapply decides_eq_refl. *)
+(*     eapply decides_and *)
+(*     decode_step. *)
+
+
+(*     apply Build_prim_and. *)
+(*     repeat decode_step. *)
+
+
+(*   (* Processes the goal by either: *) *)
+(*   match goal with *)
+(*   (* A) decomposing one of the parser combinators, *) *)
+(*   | |- _ => apply_compose *)
+(*   (* B) applying one of the rules for a base type  *) *)
+(*   | H : cache_inv_Property _ _ *)
+(*     |- appcontext [encode_decode_correct_f _ _ _ _ encode_word_Spec _ _] => *)
+(*     intros; revert H; eapply Word_decode_correct *)
+(*   | |- appcontext [encode_decode_correct_f _ _ _ _ encode_word_Spec _ _] => *)
+(*     eapply Word_decode_correct *)
+(*   | |- appcontext [encode_list_Spec] => *)
+(*     intros; eapply FixList_decode_correct *)
+(*   | |- appcontext [encode_decode_correct_f _ _ _ _ (encode_nat_Spec _) _ _] => *)
+(*     eapply Nat_decode_correct *)
+(*   | |- appcontext [encode_decode_correct_f _ _ _ _ (encode_enum_Spec _) _ _] => *)
+(*     eapply Enum_decode_correct *)
+(*   (* C) Discharging a side condition of one of the base rules *) *)
+(*   | |- NoDupVector _ => Discharge_NoDupVector *)
+(*     intros; apply Vector_predicate_rest_True *)
+(*   | _ => solve [solve_data_inv] *)
+(*   (* D) Solving the goal once all the byte string has been parsed *) *)
+(*   | _ =>  solve [simpl; intros; *)
+(*                  eapply encode_decode_correct_finish; *)
+(*                  [ build_fully_determined_type *)
+(*                  | decide_data_invariant ] ] *)
+(*   end. *)
+
+(*     decode_step. *)
+
+
+(*     apply Build_prim_and. *)
+(*     repeat decode_step. *)
+
+
+
+
+(*     build_decoder. *)
+(*     apply Build_prim_and. *)
+(*     build_decoder. *)
+(*     apply Build_prim_and. *)
+(*     { *)
+(*       build_decoder. *)
+(*       build_decoder. *)
+(*       solve_data_inv. *)
+(*       build_decoder. *)
+(*       build_decoder. *)
+(*       solve_data_inv. *)
+(*       build_decoder. *)
+(*       build_decoder. *)
+(*       solve_data_inv. *)
+(*       build_decoder. *)
+(*       build_decoder. *)
+(*       solve_data_inv. *)
+(*       build_decoder. *)
+(*       build_decoder. *)
+(*       solve_data_inv. *)
+(*       build_decoder. *)
+(*       build_decoder. *)
+(*       solve_data_inv. *)
+(*       build_decoder. *)
+(*       build_decoder. *)
+(*       solve_data_inv. *)
+(*       unfold encode_decode_correct_f; intuition eauto. *)
+(*       destruct data as [? [? [? [? [? [? [? [ ] ] ] ] ] ] ] ]. *)
+(*       unfold GetAttribute, GetAttributeRaw in *. *)
+(*       subst; simpl. *)
+(*       computes_to_inv; injections. *)
+(*       eexists; intuition eauto; simpl. *)
+(*       match goal with *)
+(*         |- ?f ?a ?b ?c = ?P => *)
+(*         let P' := (eval pattern a, b, c in P) in *)
+(*         let f' := match P' with ?f a b c => f end in *)
+(*       unify f f'; reflexivity *)
+(*       end. *)
+(*       injections; eauto. *)
+(*       eexists _; eexists _. *)
+(*     intuition eauto. *)
+(*     injections; eauto. *)
+(*     injections. *)
+(*     solve_predicate. *)
+(*     injections; eauto. *)
+(*     injections; eauto. *)
+(*     injections; eauto. *)
+(*     injections; eauto. *)
+(*     injections; eauto. *)
+(*     injections; eauto. *)
+(*     injections; eauto. *)
+(*     injections; eauto. *)
+(*     injections; eauto. *)
+(*     injections; eauto. *)
+(*     injections; eauto. *)
+(*     injections; eauto. *)
+(*     } *)
+(*     apply Build_prim_and. *)
+(*     { *)
+(*       build_decoder. *)
+(*       build_decoder. *)
+(*       solve_data_inv. *)
+(*       build_decoder. *)
+(*       build_decoder. *)
+(*       solve_data_inv. *)
+(*       build_decoder. *)
+(*       build_decoder. *)
+(*       revert H21; build_decoder. *)
+(*       shelve_inv. *)
+(*       unfold encode_decode_correct_f; intuition eauto. *)
+(*       destruct data as [? [? [? [ ] ] ] ]. *)
+(*       unfold GetAttribute, GetAttributeRaw in *. *)
+(*       subst; simpl. *)
+(*       computes_to_inv; injections. *)
+(*       eexists; intuition eauto; simpl. *)
+(*       match goal with *)
+(*         |- ?f ?a ?b ?c = ?P => *)
+(*         let P' := (eval pattern a, b, c in P) in *)
+(*         let f' := match P' with ?f a b c => f end in *)
+(*         unify f f'; reflexivity *)
+(*       end. *)
+(*       simpl in H25; injections; eauto. *)
+(*       eexists _; eexists _. *)
+(*       intuition eauto. *)
+(*       injections; eauto. *)
+(*       injections. *)
+(*       solve_predicate. *)
+(*       injections; eauto. *)
+(*       injections; eauto. *)
+(*       injections; eauto. *)
+(*       injections; eauto. *)
+(*       injections; eauto. *)
+(*     } *)
+(*     apply Build_prim_and. *)
+(*     build_decoder. *)
+(*     apply Build_prim_and. *)
+(*     { *)
+(*       build_decoder. *)
+(*       build_decoder. *)
+(*       solve_data_inv. *)
+(*       build_decoder. *)
+(*       build_decoder. *)
+(*       solve_data_inv. *)
+(*       unfold encode_decode_correct_f; intuition eauto. *)
+(*       destruct data as [? [? [ ] ] ]. *)
+(*       unfold GetAttribute, GetAttributeRaw in *. *)
+(*       subst; simpl. *)
+(*       computes_to_inv; injections. *)
+(*       eexists; intuition eauto; simpl. *)
+(*       match goal with *)
+(*         |- ?f ?a ?b ?c = ?P => *)
+(*         let P' := (eval pattern a, b, c in P) in *)
+(*         let f' := match P' with ?f a b c => f end in *)
+(*         unify f f'; reflexivity *)
+(*       end. *)
+(*       injections; eauto. *)
+(*       eexists _; eexists _. *)
+(*       intuition eauto. *)
+(*       injections; eauto. *)
+(*       injections; solve_predicate. *)
+(*       injections; eauto. *)
+(*       injections; eauto. *)
+(*       injections; eauto. *)
+(*       injections; eauto. *)
+(*       injections; solve_predicate. *)
+(*     } *)
+(*     apply Build_prim_and. *)
+(*     { build_decoder. *)
+(*       build_decoder. *)
+(*       solve_data_inv. *)
+(*       build_decoder. *)
+(*       build_decoder. *)
+(*       solve_data_inv. *)
+(*       unfold encode_decode_correct_f; intuition eauto. *)
+(*       destruct data as [? [? [ ] ] ]. *)
+(*       unfold GetAttribute, GetAttributeRaw in *. *)
+(*       subst; simpl. *)
+(*       computes_to_inv; injections. *)
+(*       eexists; intuition eauto; simpl. *)
+(*       match goal with *)
+(*         |- ?f ?a ?b ?c = ?P => *)
+(*         let P' := (eval pattern a, b, c in P) in *)
+(*         let f' := match P' with ?f a b c => f end in *)
+(*         unify f f'; reflexivity *)
+(*       end. *)
+(*       injections; eauto. *)
+(*       eexists _; eexists _. *)
+(*       intuition eauto. *)
+(*       injections; eauto. *)
+(*       injections; solve_predicate. *)
+(*       injections; eauto. *)
+(*       injections; eauto. *)
+(*       injections; eauto. *)
+(*       injections; eauto. *)
+(*       injections; solve_predicate. *)
+(*       injections; solve_predicate. *)
+(*       injections; solve_predicate. *)
+(*     } *)
+(*     apply Build_prim_and. *)
+(*     { build_decoder. *)
+(*       build_decoder. *)
+(*       solve_data_inv. *)
+(*       build_decoder. *)
+(*       build_decoder. *)
+(*       solve_data_inv. *)
+(*       unfold encode_decode_correct_f; intuition eauto. *)
+(*       destruct data as [? [? [ ] ] ]. *)
+(*       unfold GetAttribute, GetAttributeRaw in *. *)
+(*       subst; simpl. *)
+(*       computes_to_inv; injections. *)
+(*       eexists; intuition eauto; simpl. *)
+(*       match goal with *)
+(*         |- ?f ?a ?b ?c = ?P => *)
+(*         let P' := (eval pattern a, b, c in P) in *)
+(*         let f' := match P' with ?f a b c => f end in *)
+(*         unify f f'; reflexivity *)
+(*       end. *)
+(*       injections; eauto. *)
+(*       eexists _; eexists _. *)
+(*       intuition eauto. *)
+(*       injections; eauto. *)
+(*       injections; solve_predicate. *)
+(*       injections; eauto. *)
+(*       injections; eauto. *)
+(*       injections; eauto. *)
+(*       injections; eauto. *)
+(*       injections; solve_predicate. *)
+(*     } *)
+(*     apply Build_prim_and. *)
+(*     build_decoder. *)
+(*     eauto. *)
+(*     shelve_inv. *)
+(*     { unfold encode_decode_correct_f; intuition eauto. *)
+(*       destruct data as [? [? [? [? [? [ ] ] ] ] ] ]. *)
+(*       unfold GetAttribute, GetAttributeRaw in *. *)
+(*       simpl in *; subst. *)
+(*       computes_to_inv; injections. *)
+(*       eexists; intuition eauto; simpl. *)
+(*       match goal with *)
+(*       |- ?f ?a ?b ?c = ?P => *)
+(*       let P' := (eval pattern a, b, c in P) in *)
+(*       let f' := match P' with ?f a b c => f end in *)
+(*       unify f f'; reflexivity *)
+(*       end. *)
+(*       injections; eauto. *)
+(*       eexists _; eexists _. *)
+(*       intuition eauto. *)
+(*       injections; eauto. *)
+(*       solve_predicate. *)
+(*       injections; eauto. *)
+(*       injections; eauto. *)
+(*       injections; eauto. *)
+(*       injections; eauto. *)
+(*       injections; eauto. *)
+(*       injections; eauto. *)
+(*       injections; eauto. *)
+(*       injections; eauto. *)
+(*       injections; eauto. *)
+(*       injections; eauto. *)
+(*     } *)
+(*     simpl; intros; intuition eauto. *)
+(*     rewrite !app_length, H20, H21, H22. *)
+(*     reflexivity. *)
+(*     generalize data H15 x H34. *)
+(*     shelve_inv. *)
+(*     generalize data H15 x H34. *)
+(*     shelve_inv. *)
+(*     generalize data H15 x H34. *)
+(*     shelve_inv. *)
+(*     generalize data H15 x H34. *)
+(*     shelve_inv. *)
+(*     simpl; intros; intuition eauto. *)
+(*     unfold encode_decode_correct_f; intuition eauto. *)
+(*     repeat destruct data. *)
+(*     repeat destruct prim_snd. *)
+(*     unfold GetAttribute, GetAttributeRaw in *. *)
+(*     computes_to_inv. *)
+(*     repeat match goal with *)
+(*              H : context [ilist2.ith2] *)
+(*              |- _ => simpl in H *)
+(*            end. *)
+(*     repeat match goal with *)
+(*              H : ?Z *)
+(*              |- _ => match Z with context [ilist2.ith2 _ _] => simpl in H *)
+(*                      end *)
+(*            end. *)
+(*     simpl. *)
+(*     destruct prim_fst7. *)
+(*     destruct prim_snd. *)
+(*     simpl in H21; simpl in H22; simpl in H23. *)
+(*     destruct prim_snd. *)
+(*     simpl in H21. *)
+(*     destruct prim_snd. *)
+(*     simpl. *)
+(*     eexists; repeat split. *)
+(*     repeat match goal with *)
+(*              H : WS _ WO = _ |- _ => *)
+(*              let H' := fresh in *)
+(*              pose proof (f_equal (@whd _) H) as H'; simpl in H'; *)
+(*                rewrite H'; clear H' H *)
+(*            end. *)
+(*     simpl in *. *)
+(*     revert H29 H27 H28; subst. *)
+(*     injection H21; intros ? ?; subst. *)
+(*     instantiate (2 := fun al ext env' => *)
+(*                          Some *)
+(*                            ({| *)
+(*       ilist.prim_fst := _; *)
+(*       ilist.prim_snd := {| *)
+(*                          ilist.prim_fst := _; *)
+(*                         ilist.prim_snd := {| *)
+(*                                           ilist.prim_fst := _; *)
+(*                                           ilist.prim_snd := {| *)
+(*                                                   ilist.prim_fst := _; *)
+(*                                                   ilist.prim_snd := {| *)
+(*                                                   ilist.prim_fst := _; *)
+(*                                                   ilist.prim_snd := {| *)
+(*                                                   ilist.prim_fst := _; *)
+(*                                                   ilist.prim_snd := {| *)
+(*                                                   ilist.prim_fst := _; *)
+(*                                                   ilist.prim_snd := {| *)
+(*                                                   ilist.prim_fst := _; *)
+(*                                                   ilist.prim_snd := {| *)
+(*                                                   ilist.prim_fst := {| *)
+(*                                                   ilist.prim_fst := _; *)
+(*                                                   ilist.prim_snd := {| *)
+(*                                                   ilist.prim_fst := _; *)
+(*                                                   ilist.prim_snd := {| *)
+(*                                                   ilist.prim_fst := _; *)
+(*                                                   ilist.prim_snd := () |} |} |}; *)
+(*                                                   ilist.prim_snd := {| *)
+(*                                                   ilist.prim_fst := firstn proj7 al; *)
+(*                                                   ilist.prim_snd := {| *)
+(*                                                   ilist.prim_fst := firstn proj8 (skipn (proj7 + proj9) al); *)
+(*                                                   ilist.prim_snd := {| *)
+(*                                                   ilist.prim_fst := firstn proj9 (skipn proj7 al); ilist.prim_snd := () |} *)
+(*                                                    |} |} |} |} |} |} |} |} |} |} |}, *)
+(*      ext, env')). *)
+(*     simpl; intros; repeat progress f_equal. *)
+(*     eauto. *)
+(*     eauto. *)
+(*     eauto. *)
+(*     subst; apply firstn_app. *)
+(*     subst; apply firstn_skipn_app. *)
+(*     subst; rewrite skipn_app. *)
+(*     apply firstn_app. *)
+(*     injections; eauto. *)
+(*     injections; eauto. *)
+(*     eexists _; eexists _; split; split; eauto. *)
+(*     injections; simpl; eauto. *)
+(*     split. *)
+(*     simpl in H21. *)
+(*     injection H21; intros; subst. *)
+(*     unfold GetAttribute, GetAttributeRaw; simpl. *)
+(*     intuition eauto. *)
+(*     solve_predicate. *)
+(*     injections; eauto. *)
+(*     eapply H18. *)
+(*     rewrite firstn_skipn_self' in H34. *)
+(*     eauto. *)
+(*     eauto. *)
+(*     rewrite H17; clear; omega. *)
+(*     eapply H18. *)
+(*     rewrite firstn_skipn_self' in H34. *)
+(*     eauto. *)
+(*     rewrite H17; clear; omega. *)
+(*     eapply H18. *)
+(*     rewrite firstn_skipn_self' in H34. *)
+(*     eauto. *)
+(*     rewrite H17; clear; omega. *)
+(*     eapply H18. *)
+(*     rewrite firstn_skipn_self' in H34. *)
+(*     eauto. *)
+(*     rewrite H17; clear; omega. *)
+(*     revert H17 H11; clear. *)
+(*     rewrite Plus.plus_assoc; intros. *)
+(*     erewrite length_firstn_skipn_app by eauto. *)
+(*     apply H11. *)
+(*     revert H17 H10; clear. *)
+(*     rewrite Plus.plus_assoc; intros. *)
+(*     erewrite length_firstn_skipn_app' by eauto. *)
+(*     apply H10. *)
+(*     revert H17 H9; clear. *)
+(*     rewrite Plus.plus_assoc; intros. *)
+(*     erewrite length_firstn_skipn_app'' by eauto. *)
+(*     apply H9. *)
+(*     apply whd_word_1_refl. *)
+(*     apply whd_word_1_refl. *)
+(*     apply whd_word_1_refl. *)
+(*     apply whd_word_1_refl. *)
+(*     apply whd_word_1_refl. *)
+(*     revert H17; clear. *)
+(*     rewrite Plus.plus_assoc; intros. *)
+(*     eapply length_firstn_skipn_app''; eauto. *)
+(*     revert H17; clear. *)
+(*     rewrite Plus.plus_assoc; intros. *)
+(*     eapply length_firstn_skipn_app'; eauto. *)
+(*     revert H17; clear. *)
+(*     rewrite Plus.plus_assoc; intros. *)
+(*     eapply length_firstn_skipn_app; eauto. *)
+(*     eapply firstn_skipn_self'. *)
+(*     rewrite H17; omega. *)
+(*     simpl in H21. *)
+(*     injection H21; intros; subst. *)
+(*     eauto. *)
+(*     repeat instantiate (1 := fun _ => True); admit. *)
+(*     Grab Existential Variables. *)
+(*     exact 0. (* Length of the Bit-Map in WKS RDATA. *) *)
+(*     apply (@Fin.F1 _). (* RDATA Type. *) *)
+(*     apply Peano_dec.eq_nat_dec. *)
+(*     intros; destruct (weqb a a') eqn:Heq; [left | right]. *)
+(*     apply weqb_sound; eauto. *)
+(*     intro; apply weqb_true_iff in H; congruence. *)
+(*   Defined. *)
 
 End DnsPacket.
